formalization/Edka_Checked_Impl.thy
@@ -47,7 +47,7 @@ definition "edmonds_karp el s t \<equiv> do {
     None \<Rightarrow> return None
   | Some (c,ps,N) \<Rightarrow> do {
       f \<leftarrow> edka_imp c s t N ps ;
-      return (Some (N,f))
+      return (Some (c,ps,N,f))
   }
 }"
 export_code edmonds_karp checking SML
@@ -57,10 +57,11 @@ lemma network_is_impl: "Network c s t \<Longrightarrow> Network_Impl c s t" by i
 theorem edmonds_karp_correct:
   "<emp> edmonds_karp el s t <\<lambda>
       None \<Rightarrow> \<up>(\<not>ln_invar el \<or> \<not>Network (ln_\<alpha> el) s t)
-    | Some (N,fi) \<Rightarrow> 
-      \<exists>\<^sub>Af. Network_Impl.is_rflow (ln_\<alpha> el) N f fi 
-      * \<up>(Network.isMaxFlow (ln_\<alpha> el) s t f
-        \<and> ln_invar el \<and> Network (ln_\<alpha> el) s t \<and> Graph.V (ln_\<alpha> el) \<subseteq> {0..<N})
+    | Some (c,ps,N,fi) \<Rightarrow> 
+      \<exists>\<^sub>Af. Network_Impl.is_rflow c s t N f fi 
+      * \<up>(ln_\<alpha> el = c \<and> is_pred_succ ps c
+        \<and> Network.isMaxFlow c s t f
+        \<and> ln_invar el \<and> Network c s t \<and> Graph.V c \<subseteq> {0..<N})
   >\<^sub>t"
   unfolding edmonds_karp_def
   using prepareNet_correct[of el s t]
@@ -78,18 +79,217 @@ theorem
   fixes el defines "c \<equiv> ln_\<alpha> el"
   shows "<emp> edmonds_karp el s t <\<lambda>
       None \<Rightarrow> \<up>(\<not>ln_invar el \<or> \<not>Network c s t)
-    | Some (N,cf) \<Rightarrow> 
+    | Some (_,_,N,cf) \<Rightarrow> 
       \<up>(ln_invar el \<and> Network c s t \<and> Graph.V c \<subseteq> {0..<N})
-    * (\<exists>\<^sub>Af. is_rflow c N f cf * \<up>(Network.isMaxFlow c s t f))>\<^sub>t"
+    * (\<exists>\<^sub>Af. is_rflow c s t N f cf * \<up>(Network.isMaxFlow c s t f))>\<^sub>t"
 text_raw \<open>}%EndSnippet\<close>
   unfolding c_def is_rflow_def
   by (sep_auto heap: edmonds_karp_correct[of el s t] split: option.split)
 
 end
 
+subsection \<open>Usage Example: Computing Maxflow Value \<close>
+text \<open>We implement a function to compute the value of the maximum flow.\<close>
+
+
+lemma (in Network) ps_s_is_incoming:
+  assumes "is_pred_succ ps c"
+  shows "E``{s} = set (ps s)"
+  using assms no_incoming_s
+  unfolding is_pred_succ_def
+  by auto
+  
+context RGraph begin
+
+  lemma val_by_adj_map:
+    assumes "is_pred_succ ps c"
+    shows "f.val = (\<Sum>v\<in>set (ps s). c (s,v) - cf (s,v))"
+  proof -
+    have "f.val = (\<Sum>v\<in>E``{s}. c (s,v) - cf (s,v))"
+      unfolding f.val_alt
+      by (simp add: sum_outgoing_pointwise f_def flow_of_cf_def)
+    also have "\<dots> = (\<Sum>v\<in>set (ps s). c (s,v) - cf (s,v))"  
+      by (simp add: ps_s_is_incoming[OF assms])
+    finally show ?thesis . 
+  qed  
+      
+end
+
+
+context Network 
+begin
+
+  definition "get_cap e \<equiv> c e"
+  definition (in -) get_ps :: "(node \<Rightarrow> node list) \<Rightarrow> node \<Rightarrow> node list" 
+    where "get_ps ps v \<equiv> ps v"
+
+  definition "compute_flow_val ps cf \<equiv> do {
+      let succs = get_ps ps s;
+      setsum_impl 
+      (\<lambda>v. do {
+        let csv = get_cap (s,v);
+        cfsv \<leftarrow> cf_get cf (s,v);
+        return (csv - cfsv)
+      }) (set succs)
+    }"
+
+  lemma (in RGraph) compute_flow_val_correct:
+    assumes "is_pred_succ ps c"
+    shows "compute_flow_val ps cf \<le> (spec v. v = f.val)"
+    unfolding val_by_adj_map[OF assms]
+    unfolding compute_flow_val_def cf_get_def get_cap_def get_ps_def
+    apply (refine_vcg setsum_imp_correct)
+    apply (vc_solve simp: s_node)
+    unfolding ps_s_is_incoming[symmetric, OF assms] 
+    by (auto simp: V_def)
+
+  text \<open>For technical reasons (poor foreach-support of Sepref tool), 
+    we have to add another refinement step: \<close>  
+  definition "compute_flow_val2 ps cf \<equiv> (do {
+    let succs = get_ps ps s;
+    nfoldli succs (\<lambda>_. True)
+     (\<lambda>x a. do {
+           b \<leftarrow> do {
+               let csv = get_cap (s, x);
+               cfsv \<leftarrow> cf_get cf (s, x);
+               return (csv - cfsv)
+             };
+           return (a + b)
+         })
+     0
+  })"  
+
+  lemma (in RGraph) compute_flow_val2_correct:
+    assumes "is_pred_succ ps c"
+    shows "compute_flow_val2 ps cf \<le> (spec v. v = f.val)"
+  proof -
+    have [refine_dref_RELATES]: "RELATES (\<langle>Id\<rangle>list_set_rel)" 
+      by (simp add: RELATES_def)
+    show ?thesis
+      apply (rule order_trans[OF _ compute_flow_val_correct[OF assms]])
+      unfolding compute_flow_val2_def compute_flow_val_def setsum_impl_def
+      apply (rule refine_IdD)
+      apply (refine_rcg LFO_refine bind_refine')
+      apply refine_dref_type
+      apply vc_solve
+      using assms
+      by (auto 
+          simp: list_set_rel_def br_def get_ps_def is_pred_succ_def 
+          simp: refine_pw_simps)
+  qed    
+    
+
+
+end
+
+context Edka_Impl begin
+  term is_ps
+
+  lemma [sepref_import_param]: "(c,PR_CONST get_cap) \<in> Id\<times>\<^sub>rId \<rightarrow> Id" 
+    by (auto simp: get_cap_def)
+  lemma [def_pat_rules]: 
+    "Network.get_cap$c \<equiv> UNPROTECT get_cap" by simp
+  sepref_register 
+    "PR_CONST get_cap" "node\<times>node \<Rightarrow> capacity_impl"
+
+  lemma [sepref_import_param]: "(get_ps,get_ps) \<in> Id \<rightarrow> Id \<rightarrow> \<langle>Id\<rangle>list_rel" 
+    by (auto simp: get_ps_def intro!: ext)
+
+  schematic_lemma compute_flow_val_imp:
+    fixes ps :: "node \<Rightarrow> node list" and cf :: "capacity_impl graph"
+    notes [id_rules] = 
+      itypeI[Pure.of ps "TYPE(node \<Rightarrow> node list)"]
+      itypeI[Pure.of cf "TYPE(capacity_impl i_mtx)"]
+    notes [sepref_import_param] = IdI[of N] IdI[of ps]
+    shows "hn_refine 
+      (hn_ctxt (is_mtx N) cf cfi)
+      (?c::?'d Heap) ?\<Gamma> ?R (compute_flow_val2 ps cf)"
+    unfolding compute_flow_val2_def
+    using [[id_debug, goals_limit = 1]]
+    by sepref_keep
+      
+  concrete_definition (in -) compute_flow_val_imp for c s N ps cfi
+    uses Edka_Impl.compute_flow_val_imp
+
+  prepare_code_thms (in -) compute_flow_val_imp_def
+
+end
+
+context Network_Impl begin
+
+lemma compute_flow_val_imp_correct_aux: 
+  assumes VN: "Graph.V c \<subseteq> {0..<N}"
+  assumes ABS_PS: "is_pred_succ ps c"
+  assumes RG: "RGraph c s t cf"
+  shows "
+    <is_mtx N cf cfi> 
+      compute_flow_val_imp c s N ps cfi
+    <\<lambda>v. is_mtx N cf cfi * \<up>(v = Flow.val c s (flow_of_cf cf))>\<^sub>t"
+proof -
+  interpret rg!: RGraph c s t cf by fact
+
+  have EI: "Edka_Impl c s t N" by unfold_locales fact
+  from hn_refine_ref[OF 
+      rg.compute_flow_val2_correct[OF ABS_PS] 
+      compute_flow_val_imp.refine[OF EI], of cfi]
+  show ?thesis
+    apply (simp add: hn_ctxt_def pure_def hn_refine_def rg.f_def)
+    apply (erule cons_post_rule)
+    apply sep_auto
+    done
+qed
+
+lemma compute_flow_val_imp_correct: 
+  assumes VN: "Graph.V c \<subseteq> {0..<N}"
+  assumes ABS_PS: "is_pred_succ ps c"
+  shows "
+    <is_rflow N f cfi> 
+      compute_flow_val_imp c s N ps cfi
+    <\<lambda>v. is_rflow N f cfi * \<up>(v = Flow.val c s f)>\<^sub>t"
+  apply (rule hoare_triple_preI)  
+  apply (clarsimp simp: is_rflow_def)
+  apply vcg
+  apply (rule cons_rule[OF _ _ compute_flow_val_imp_correct_aux[where cfi=cfi]])
+  apply (sep_auto simp: VN ABS_PS)+
+  done
+
+end
+
+
+definition "edmonds_karp_val el s t \<equiv> do {
+  r \<leftarrow> edmonds_karp el s t;
+  case r of
+    None \<Rightarrow> return None
+  | Some (c,ps,N,cfi) \<Rightarrow> do {
+      v \<leftarrow> compute_flow_val_imp c s N ps cfi;
+      return (Some v)
+    } 
+}"
+
+theorem edmonds_karp_val_correct:
+  "<emp> edmonds_karp_val el s t <\<lambda>
+    None \<Rightarrow> \<up>(\<not>ln_invar el \<or> \<not>Network (ln_\<alpha> el) s t)
+  | Some v \<Rightarrow> \<up>(\<exists>f N. 
+          ln_invar el \<and> Network (ln_\<alpha> el) s t 
+        \<and> Graph.V (ln_\<alpha> el) \<subseteq> {0..<N}
+        \<and> Network.isMaxFlow (ln_\<alpha> el) s t f
+        \<and> v = Flow.val (ln_\<alpha> el) s f)  
+        >\<^sub>t"
+  unfolding edmonds_karp_val_def
+  by (sep_auto 
+    intro: network_is_impl
+    heap: edmonds_karp_correct Network_Impl.compute_flow_val_imp_correct)      
+
+
+subsection \<open>Exporting Code\<close>
+
+(*
 (* TODO: Justify this by abstract definition + refinement *)  
 text \<open>Unverified function to extract the maximum flow value.\<close>
-definition get_flow :: "capacity_impl graph \<Rightarrow> nat \<Rightarrow> Graph.node \<Rightarrow> capacity_impl mtx \<Rightarrow> capacity_impl Heap" where
+definition get_flow 
+  :: "capacity_impl graph \<Rightarrow> nat \<Rightarrow> Graph.node \<Rightarrow> capacity_impl mtx 
+    \<Rightarrow> capacity_impl Heap" 
+  where
   "get_flow c N s fi \<equiv> do {
     imp_nfoldli ([0..<N]) (\<lambda>_. return True) (\<lambda>v cap. do {
       let csv = c (s,v);
@@ -98,10 +298,11 @@ definition get_flow :: "capacity_impl graph \<Rightarrow> nat \<Rightarrow> Grap
       return (cap + fsv)
     }) 0
   }"
-
+*)
 
 export_code nat_of_integer integer_of_nat int_of_integer integer_of_int
-  edmonds_karp edka_imp edka_imp_tabulate edka_imp_run prepareNet get_flow
+  edmonds_karp edka_imp edka_imp_tabulate edka_imp_run prepareNet
+  compute_flow_val_imp edmonds_karp_val
   in SML_imp 
   module_name Fofu 
   file "evaluation/fofu-SML/Fofu_Export.sml"  
